Update Addition.fst

SkipList/FStar/Addition.fst
@@ -6,3 +6,48 @@ open IntegerExpansion
 val computeMaxLevel: elements: nat{elements > 1} -> Tot(nat)
 let computeMaxLevel elements = 
     IntegerExpansion.log2Tot elements
+
+type skipList 'a =
+|Mk: value : 'a -> levels: int -> a:list(skipList 'a) -> skipList 'a
+|MkRoot : skipList 'a
+
+type sca 'a =
+| Mk: memory : list ((option skipList 'a)* (option skipList 'a))
+
+type sca 'a = 
+| Mk : memoryFrom : list (option skipList 'a ) -> memoryTo : list (option skipList 'a )-> sca 'a
+
+val generateSCA: level:nat -> sca 'a
+let generateSCA sca = 
+	let rec f c lstFrom lstTo = 
+	if c > level then 
+		let lstFrom = FStar.List.Tot.append lstFrom [None] in 
+		let lstTo = FStar.List.Tot.append lstTo [None] in 
+		f (c+1) lstFrom lstTo 
+	else
+		Mk lstFrom lstTo	
+
+
+assume val generateLevel: maxLevel : nat -> nat
+assume val buildLevelTree : sl: skipList 'a -> sca 'a -> sca 'a
+
+val scaReplace: f: option(skipList 'a) -> t: option (skipList 'a )->
+	level : nat -> sca: sca 'a -> sca 'a
+let scaReplace = 
+ 	match sca with 
+ 	| Mk memoryFrom memoryTo ->
+ 	let memoryFrom =  ListExpansion.replace memoryFrom f level in 
+ 	let memoryTo = ListExpansion.replace memoryTo f level in 
+ 	Mk memoryFrom memoryTo
+
+val createLeaf : sca : sca 'a -> sl:skipList 'a ->value:'a ->  skipList 'a
+let createLeaf sca sl value =
+
+
+val insert: skipList 'a ->level:nat ->  skipList 'a
+let insert sl = 
+	let sca = generateSCA in 
+	let level = generateLevel level in 
+	match sl with 
+	| MkRoot -> createLeaf sca sl level
+	| Mk v l a -> let sca = buildLevelTree sl sca in createLeaf sca sl level
